\documentclass{article}
\usepackage{amsmath} % for equation environments
\usepackage{amssymb} % for extra math symbols
\usepackage{geometry} % optional: better margins
\geometry{margin=1in}
\pagestyle{empty}

\begin{document}

\begin{equation*}
    E_{\text{GFN2-xTB}} = E_{\text{rep}} + E_{\text{disp}} + E_{\text{EHT}} + E_{\text{IES+IXC}} + E_{\text{AES}} + E_{\text{AXC}} + G_{\text{Fermi}}
\end{equation*}

\begin{equation*}
    E_{\mathrm{EHT}} = \sum_i n_i \langle \psi_i | \hat{H}_0 | \psi_i \rangle
    = \sum_{\kappa} \sum_{\lambda} P_{\kappa \lambda} H_{\kappa \lambda}
\end{equation*}

\begin{equation*}
    H_{\kappa\lambda} = k_{ll'} \cdot \frac{1}{2}(H_{\kappa\kappa} + H_{\lambda\lambda}) \cdot S_{\kappa\lambda}
    \left( \frac{2 \sqrt{\zeta_\kappa \zeta_\lambda}}{\zeta_\kappa + \zeta_\lambda} \right)^{1/2}
    \left( 1 + k_{\mathrm{EN}} \Delta \mathrm{EN}_{AB}^2 \right) \Pi(R_{AB,ll'})
    \qquad (\kappa \in l \in A, \; \lambda \in l' \in B)
\end{equation*}

\begin{equation*}
    E_{\mathrm{rep}} = \sum_{AB}
    \frac{Y_A^{\mathrm{eff}} Y_B^{\mathrm{eff}}}{R_{AB}}
    e^{ -\left( \alpha_A \alpha_B \right)^{1/2} (R_{AB})^{k_{\mathrm{rep}}} }
\end{equation*}

\begin{equation*}
    \Delta_{\text{dist}} = \left\| D^{\text{xTB}} - D^{\text{DFT}} \right\|_F
    = \sqrt{ \sum_{i=1}^{N} \sum_{j=1}^{N} \left( D_{ij}^{\text{xTB}} - D_{ij}^{\text{DFT}} \right)^2 }
\end{equation*}

\begin{equation*}
    F_{\text{max}} = \max_{i \in \{1, \ldots, N\}} \left\| \mathbf{F}_i \right\|_2
    = \max_{i} \sqrt{F_{ix}^2 + F_{iy}^2 + F_{iz}^2}
\end{equation*}


\begin{equation*}
    x^{(t+1)} = x^{(t)} - \eta \cdot \nabla f(x^{(t)}), \quad \text{where} \quad
    \frac{\partial f}{\partial x_i} \approx \frac{f(x^{(t)} + \epsilon e_i) - f(x^{(t)} - \epsilon e_i)}{2\epsilon}
\end{equation*}

\begin{equation*}
    \psi_i = \sum_{\kappa}^{N_{\text{AO}}} c_{\kappa i} \, \phi_{\kappa}(\zeta_{\kappa}, \text{STO-}m\text{G})
\end{equation*}

\begin{equation*}
    \begin{aligned}
        E_{\text{EHT}} & = \sum_{i} n_i \langle \psi_i | \hat{H}_0 | \psi_i \rangle
        = \sum_{\kappa} \sum_{\lambda} \sum_{i} n_i c_{\kappa i} c_{\lambda i}
        \langle \phi_{\lambda} | \hat{H}_0 | \phi_{\kappa} \rangle                                 \\
                       & \equiv \sum_{\kappa} \sum_{\lambda} P_{\kappa \lambda} H_{\lambda \kappa}
    \end{aligned}
\end{equation*}

\begin{equation*}
    \text{MAE} = \frac{1}{N} \sum_{i=1}^{N} \left| E_i^{\text{xTB}} - E_i^{\text{DFT}} \right|
\end{equation*}

\begin{enumerate}
    \item $k_{\text{rep}}$
    \item $k_{\text{sd}}$
    \item $k_{\text{pd}}$
    \item $k_{\text{ss}}$
    \item $k_{\text{pp}}$
\end{enumerate}


\end{document}
